src/coq/CFG.v
@@ -9,13 +9,14 @@
  ---------------------------------------------------------------------------- *)
 
 Require Import ZArith List String Omega.
-Require Import Vellvm.AstLib Vellvm.Ollvm_ast Vellvm.Dom.
+Require Import Vellvm.AstLib Vellvm.Ollvm_ast.
 Require Import Vellvm.Classes.
+Require Import Vellvm.Util.
 Import ListNotations.
 
-Definition pt := instr_id.
-
 (* program counter is a function plus instruction id ------------------------ *)
+
+Definition pt := instr_id.
 
 Record pc :=
   mk_pc {
@@ -23,9 +24,8 @@ Record pc :=
       ins : pt;
     }.
 
-Definition string_of_pc p : string :=
-  "@" ++ (string_of_raw_id (fn p)) ++ ":" ++ (string_of_instr_id (ins p)).
-
+Instance string_of_pc : StringOf pc :=
+  fun p => "@" ++ (string_of_raw_id (fn p)) ++ ":" ++ (string_of_instr_id (ins p)).
 
 Require Import Equalities.
 Module PC <: UsualDecidableTypeFull.
@@ -72,266 +72,20 @@ Record cfg := mkCFG
                           including globals and local function parameters *)
 }.
 
-(* When does a cfg program point define a given local_id. *)
-Definition pt_defines (p:pt) (lid:local_id) :=
-  match p with
-  | IId id => if id == lid then True else False
-  | IVoid _ => False
-  end.
+(* An mcfg is a module where each function body has been converted to a cfg *)
+Definition mcfg : Set := modul cfg.
 
-(* Which identifiers does an instruction use? *)
-Fixpoint value_uses (v:value) : list ident :=
-  match v with
-  | SV (VALUE_Ident _ id) => [id]
-  | SV (VALUE_Integer _ _)
-  | SV (VALUE_Float _ _ )
-  | SV (VALUE_Bool _ _)
-  | SV (VALUE_Null _)
-  | SV (VALUE_Zero_initializer _)
-  | SV (VALUE_Cstring _ _)
-  | SV (VALUE_None _)
-  | SV (VALUE_Undef _) => []
+Definition find_defn {X:Set} (fid:function_id) (d:definition X) : option (definition X) :=
+  if (ident_of d) == (ID_Global fid) then Some d else None.
 
-  | SV (VALUE_Struct _ l)
-  | SV (VALUE_Packed_struct _ l)
-  | SV (VALUE_Array _ l)
-  | SV (VALUE_Vector _ l) => List.flat_map (fun x => value_uses (snd x)) l
-  | SV (OP_IBinop _ _ _ v1 v2) 
-  | SV (OP_ICmp _ _ _ v1 v2)
-  | SV (OP_FBinop _ _ _ _ v1 v2) 
-  | SV (OP_FCmp _ _ _ v1 v2) => (value_uses v1) ++ (value_uses v2)
-  | SV (OP_Conversion _ _ _ v _) => value_uses v
-  | SV (OP_GetElementPtr _ _ (_,ptr) idxs) => (value_uses ptr) ++ (List.flat_map (fun x => value_uses (snd x)) idxs)
-  | SV (OP_ExtractElement _  (_,vec) (_,idx)) => (value_uses vec) ++ (value_uses idx)
-  | SV (OP_InsertElement _ (_,vec) (_,elt) (_,idx)) => (value_uses vec) ++ (value_uses elt) ++ (value_uses idx)
-  | SV (OP_ShuffleVector _ (_, vec1) (_,vec2) (_,idxmask)) => (value_uses vec1) ++ (value_uses vec2) ++ (value_uses idxmask)
-  | SV (OP_ExtractValue _ (_,vec) _) => value_uses vec
-  | SV (OP_InsertValue _ (_,vec) (_,elt) _) => (value_uses vec) ++ (value_uses elt)
-  | SV (OP_Select _ (_,cnd) (_,v1) (_,v2)) => (value_uses cnd) ++ (value_uses v1) ++ (value_uses v2)
-  end.
+Definition find_function {X:Set} (CFG : modul X) (fid:function_id) : option (definition X) :=
+  find_map (find_defn fid) (m_definitions CFG).
 
-Definition tvalue_uses (tv:tvalue) : list ident := value_uses (snd tv).
-
-(* over-approximation: may include the same identifier more than once *)
-Definition instr_uses (i:instr) : (list ident) :=
-  match i with
-  | INSTR_Op op => value_uses op                         
-  | INSTR_Call (_, fid) args => [fid] ++ (List.flat_map tvalue_uses args)
-  | INSTR_Phi  t args => List.flat_map (fun x => value_uses (snd x)) args
-  | INSTR_Alloca t None align => []
-  | INSTR_Alloca t (Some tv) align => tvalue_uses tv
-  | INSTR_Load  volatile t ptr align => tvalue_uses ptr
-  | INSTR_Store volatile val ptr align => (tvalue_uses val) ++ (tvalue_uses ptr)
-  | INSTR_Fence 
-  | INSTR_AtomicCmpXchg
-  | INSTR_AtomicRMW
-  | INSTR_Unreachable
-  | INSTR_VAArg
-  | INSTR_LandingPad => []
-  end.
-
-Definition terminator_uses (t:terminator) : list ident :=
-  match t with
-  | TERM_Ret tv => tvalue_uses tv
-  | TERM_Ret_void => []
-  | TERM_Br tv _ _ => tvalue_uses tv
-  | TERM_Br_1  _ => []
-  | TERM_Switch  tv _ brs => (tvalue_uses tv) ++ (List.flat_map (fun x => tvalue_uses (fst x)) brs)
-  | TERM_IndirectBr tv _ => tvalue_uses tv
-  | TERM_Resume tv => tvalue_uses tv
-  | TERM_Invoke (_,fid) args _ _ => [fid] ++ (List.flat_map tvalue_uses args)
-  end.
-
-(* Which labels does a terminator mention *)
-Definition lbls (t:terminator) : list block_id :=
-  match t with
-  | TERM_Ret _        
-  | TERM_Ret_void   => []
-  | TERM_Br _ l1 l2 => [l1; l2] 
-  | TERM_Br_1 l => [l] 
-  | TERM_Switch _ l brs => l::(List.map (fun x => snd x) brs)
-  | TERM_IndirectBr _ brs => brs
-  | TERM_Resume _    => []
-  | TERM_Invoke  _ _ l1 l2 => [l1; l2] 
-  end.
-
-
-(* Well-formed SSA-form CFGs 
-   - the initial pt denotes a command  
-   - fallthrough closure: each fallthrough pt maps to a command 
-   - jump closure: each label used in a terminator leads to a
-     block within the same function body.
-   - every use of an identifier is dominated by the id's definition
-   - no identifier is defined multiple times
-*)
-Definition pt_exists (CFG : cfg) (p:pt) : Prop :=
-  exists cmd, (code CFG p) = Some cmd.
-
-
-(** Edge relation *)
-Inductive edge_pt (g:cfg) : pt -> pt -> Prop :=
-| edge_pt_S : forall p i q,
-    (code g) p = Some (Step i q) ->
-    edge_pt g p q
-| edge_pt_J : forall p b t l q xs r,
-    (code g) p = Some (Jump b t) ->
-    In l (lbls t) ->
-    (phis g) l = Some (Phis q xs r) ->
-    edge_pt g p q.
-
-(** *** GRAPH instance for dominance calculation *)
-(** Graph of program points *)
-
-Module PtGraph <: GRAPH.
-  Definition t := cfg.
-  Definition V := pt.
-  Definition entry g := init g.
-  Definition edge := edge_pt.
-  Definition mem := pt_exists.
-End PtGraph.
-
-Module Export Dom := Dom.Spec PtGraph.
-
-
-(** *** Definitions for Well-formed SSA programs. *)
-
-(** Most of the LLVM instructions define the uid associated
-  with their program point.  Some (like [store], [void] calls, and the [terminator]s)
-  do not. *)
-Definition def_at_pt (g:cfg) (p:pt) (lid:local_id) : Prop :=
-  pt_exists g p /\ pt_defines p lid.
-
-(** The definition of id dominates its use at point pt *)
-Inductive well_scoped_use_at_pt (g:cfg) (p:pt) : ident -> Prop :=
-| ws_global : forall id, In id (glbl g) -> pt_exists g p -> well_scoped_use_at_pt g p id
-| ws_local : forall lid p', def_at_pt g p' lid -> SDom g p' p -> well_scoped_use_at_pt g p (ID_Local lid).
-
-(** All uses of a [uid] must be strictly dominated by their definitions. *)
-Definition wf_use (g:cfg) (ids:list ident) (p:pt) : Prop :=
-  forall id, In id ids -> well_scoped_use_at_pt g p id.
-
-
-(** *** Well-formed phi nodes *)
-(**  Consider [ %x = phi [lbl1:v1, ...,lbln:vn] ].  This is well formed
-     when every predecessor block with terminator program point p' 
-     has a label associated with value v.  Moreover, if v uses an id then
-     the definition of the uid strictly dominates p'.
-*)
-
-Definition wf_phi_args (g:cfg) (entry:pt) (args:list (block_id * value)) :=
-  forall pred, edge_pt g pred entry ->
-          exists b t, (code g) pred = Some (Jump b t) /\
-                 exists v, In (b,v) args /\ wf_use g (value_uses v) pred.
-
-Inductive wf_phis (CFG : cfg) (entry:pt) (q : pt) : pt -> list (local_id * instr) -> Prop :=
-| wf_phis_nil : pt_exists CFG q ->
-                wf_phis CFG entry q q []
-
-| wf_phis_cons :
-    forall p p' x t args rest,
-    (code CFG p) = Some (Step (INSTR_Phi t args) p') ->
-    wf_phi_args CFG entry args ->
-    wf_phis CFG entry q p' rest ->
-    wf_phis CFG entry q p ((x, INSTR_Phi t args) :: rest) .
-
-Inductive wf_cmd (g:cfg) (p:pt) : cmd -> Prop :=
-| wf_step : forall (i:instr) (q:pt)
-              (Hq : pt_exists g q)
-              (Huse: wf_use g (instr_uses i) p),
-    wf_cmd g p (Step i q)
-
-| wf_jump : forall (bn:block_id) (t:terminator)
-              (Huse: wf_use g (terminator_uses t) p)
-              (Hlbls: Forall (fun tgt => exists p', exists xs, exists q,
-                             (phis g tgt) = Some (Phis p' xs q) 
-                             /\ wf_phis g p' q p' xs
-                      )
-                      (lbls t)),
-    wf_cmd g p (Jump bn t).
-
-
-(* TODO: do we have to worry about locals shadowing function parameters? 
-   Could add: forall lid, In (ID_Local lid) (glbl CFG) -> (code CFG) (IId lid) = None
-
-   - also, somewhere probably need that globals and function parameters are distinct
- *)
-
-Definition wf_cfg (CFG : cfg) : Prop :=
-  pt_exists CFG (init CFG)
-  /\ forall p, ~ edge_pt CFG p (init CFG)            
-  /\ (forall p cmd, (code CFG p) = Some cmd -> wf_cmd CFG p cmd)
-.
-
-(*
-  Definition wf_phi_args (g:Cfg.t) (i:insn) (p:pc) : Prop :=
-    forall pred, edge_pt g pred (entry_of_pc p) ->
-      (exists v, In (lbl_of pred, v) (insn_phis i)) /\
-      (forall uid, In (lbl_of pred, val_uid uid) (insn_phis i) -> 
-          uid_sdom_pc g uid pred).
-
-  Definition wf_phi_pred (g:Cfg.t) (i:insn) (p:pc) : Prop :=
-    forall l v, In (l, v) (insn_phis i) ->
-      (exists pred, edge_pt g pred (entry_of_pc p) /\ lbl_of pred = l).
-
-  Definition wf_phi (g:Cfg.t) (i:insn) (p:pc) : Prop :=
-    is_phi i -> wf_phi_args g i p
-             /\ wf_phi_pred g i p
-             /\ insn_phis i <> [].
-
-  (** *** Well-formed instructions *)
-
-  Inductive wf_insn (g:Cfg.t) : insn -> pc -> Prop :=
-  | wf_insn_intro : forall i p,
-      wf_use g i p ->
-      wf_lbl g i ->
-      wf_phi g i p ->
-      wf_insn g i p.
-
-  Inductive wf_prog (g:Cfg.t) : Prop :=
-  | wf_prog_intro : forall
-      (Hwfcfg : wf_cfg g)
-      (Hwfis : forall p i, insn_at_pc g p i -> wf_insn g i p)
-      (Hwftmn : forall p' i, tmn_pc g p' -> insn_at_pc g p' i -> is_tmn i)
-      (Hwfentry : forall p, ~ edge_pt g p (block_entry (entry_block g))),
-      wf_prog g.
-
-
-            
-Lemma wf_cfg_edge_pt : forall g p1 p2,
-    wf_cfg g -> pt_exists g p1 -> edge_pt g p1 p2 -> pt_exists g p2.
-Proof.
-  intros g p1 p2 H H0 H1.
-  destruct H as [Hinit [HStep HJump]].
-  inversion H1; subst.
-  - eapply HStep. apply H.
-  - apply HJump in H.
-    eapply Forall_forall in H.
-    Focus 2. apply H2.
-    destruct H as [p' [xs [q [Ha [Hb [Hc Hd]]]]]].
-    rewrite H3 in Ha. inversion Ha. subst.
-    induction Hc.
-    * exact Hd.
-    * exists (Step (INSTR_Phi t0 args) p').
-      exact H.
-Qed.      
-*)
-
-
-
-
+Definition fetch (CFG : mcfg) (p:pc) :=
+  'fdefn <- find_function CFG (fn p);
+  (code (df_instrs fdefn) (ins p)).
 
 (* creating CFGs from syntax ------------------------------------------------ *)
-         
-Fixpoint lookup_function_definition ets f : option definition :=
-  match ets with
-  | [] => None
-  | (TLE_Definition d) :: ts =>
-    if (dc_name (df_prototype d)) == f then
-      Some d
-    else
-      lookup_function_definition ts f
-  | _ :: ts => lookup_function_definition ts f
-  end.
 
 Definition fallthrough term_id (is : list (instr_id * instr)) : instr_id :=
   match is with
@@ -392,43 +146,43 @@ match bs with
     end
   end.
 
-Definition code_of_definition (d:definition) (p:pt) : option cmd :=
+Definition code_of_definition (d:definition (list block)) (p:pt) : option cmd :=
   cmd_from_blocks p (df_instrs d).
   
-
-Definition blks_of_definition (d:definition) block_id : option pt :=
+Definition blks_of_definition (d:definition (list block)) block_id : option pt :=
   'b <- lookup_block (df_instrs d) block_id;
   Some (fallthrough (blk_term_id b) (blk_instrs b)).
 
-Definition phis_of_definition (d:definition) block_id : option block_entry :=
+Definition phis_of_definition (d:definition (list block)) block_id : option block_entry :=
   'b <- lookup_block (df_instrs d) block_id;
   block_to_phis b.
 
-Definition cfg_of_definition (g:list ident) (d:definition) : option cfg :=
+Definition cfg_of_definition (g:list ident) (d:definition (list block)) : option cfg :=
   'init <- init_of_definition d;
+    let args := List.map (fun x => ID_Local x) (df_args d) in
     Some {| init := init;
             code := code_of_definition d;
             phis := phis_of_definition d;
-            glbl := g;
+            glbl := g++args;
          |}.
-            
-Definition fcfg := function_id -> option (list local_id * cfg).
 
-Definition globals_of (tle : toplevel_entity) : list ident :=
-  match tle with
-  | TLE_Declaration d => [ID_Global (dc_name d)]
-  | TLE_Definition d => [ID_Global (dc_name (df_prototype d))]
-  | TLE_Global g => [ID_Global (g_ident g)]
-  | _ => []
-  end.
 
-Definition globals (ets : list toplevel_entity) : list ident :=
-  List.fold_right (fun tle acc => (globals_of tle) ++ acc) [] ets.
-
-Fixpoint entities_to_funs ets fid : option (list local_id * cfg) :=
-  'd <- lookup_function_definition ets fid;
-    let args := List.map (fun x => ID_Local x) (df_args d) in
-    let g := globals ets in
-    'cfg <- cfg_of_definition (g++args) d;
-    Some (df_args d, cfg).
+Definition mfg_of_modul (m:modul (list block)) : option mcfg :=
+  let glbls := globals m in
+  'defns <- map_option
+                (fun d =>
+                   'cfg <- cfg_of_definition glbls d;
+                     Some {|
+                       df_prototype := df_prototype d;
+                       df_args := df_args d;
+                       df_instrs := cfg
+                       |}) (m_definitions m) ;
+  Some {|
+    m_name := m_name m;
+    m_target := m_target m;
+    m_datalayout := m_datalayout m;
+    m_globals := m_globals m;
+    m_declarations := m_declarations m;
+    m_definitions := defns
+  |}.
 
